Prove Equality from E.Mendelson

Ackermann.v
@@ -15,7 +15,6 @@ Module PredSymb : UsualDecidableTypeFull := PeanoNat.Nat.
 Module X := Provability_mod SetVars FuncSymb PredSymb.
 Export X.
 Module Facts := BoolEqualityFacts SetVars.
-Check substF.
 
 (*Local Notation SetVars := SetVars.t (only parsing).
 Local Notation FuncSymb := FuncSymb.t (only parsing).
@@ -26,14 +25,21 @@ Import VectorNotations.
 
 Section inf_sec.
 Context (en:nat->PredSymb.t) (enInj: forall x1 x2, en x1 = en x2 -> x1=x2).
+Context (es:nat->SetVars.t) (esInj: forall x1 x2, es x1 = es x2 -> x1=x2).
 (*Module Facts := BoolEqualityFacts SetVars.*)
+(*Notation "( a '==' b )" :=
+(Atom {| ps := en 0; psv := 2 |} [a:Terms; b:Terms]).*)
 Notation "( a '==' b )" :=
-(Atom {| ps := en 0; psv := 2 |} [a:Terms; b:Terms]).
+(Atom {| ps := en 0; psv := 2 |} 
+(@Vector.cons Terms a 1 (@Vector.cons Terms b 0 (@Vector.nil Terms)))
+).
+Coercion es:nat>->SetVars.t.
+
 Notation "( a 'e.' b )" := (Atom {| ps := en 1; psv := 2 |} [a:Terms; b:Terms]).
 
 Inductive AxiomAST : Fo -> Type :=
 | aPC  :> forall {A}, (AxiomH A) -> (AxiomAST A)
-| aeq1 : forall (x:SetVars.t), AxiomAST (x == x)
+| aeq1 : forall (x:SetVars.t), AxiomAST (Fora 0 (0 == 0))
 (*AxiomAST (Atom (MPSV (en 0) 2) [FVC x ; FVC x])*)
 | aeq2 : forall (x y:SetVars.t) (f r:Fo)
 (H:substF y x f = Some r)
@@ -45,7 +51,6 @@ Inductive AxiomAST : Fo -> Type :=
    (MPSV 1 2) - \in
 *)
 (*Check AxiomAST (Ha1 Bot Bot). ? *)
-Check Vector.cons .
 (*Notation "( a '==' b )" := (Atom (MPSV (en 0) 2) [FVC a ; FVC b]).*)
 (*Notation "( a '==' b )" := (Atom (MPSV (en 0) 2) [a:Terms ; b:Terms]).
 Notation "( a 'e.' b )" := (Atom (MPSV (en 1) 2) [a:Terms ; b:Terms]).
@@ -53,26 +58,29 @@ Notation "( a 'e.' b )" := (Atom (MPSV (en 1) 2) [a:Terms ; b:Terms]).
 
 
 (* Provability in Ackermann set theory *)
-Definition APR := @GPR AxiomAST.
+Definition APR := GPR AxiomAST.
 (* Mendelson p.102/447 *)
 (*Coercion FVC : SetVars.t >-> Terms.*)
 (*Coercion Q : (Vector.t SetVars.t n) >-> (Vector.t Terms n).*)
-Theorem J (y:SetVars.t): Terms.
-exact y. Defined.
-Definition p2_23_a ctx (t:Terms) (x:SetVars.t): APR ctx (t == t).
+Theorem J (y:SetVars.t): Terms. exact y. Defined.
 
 Theorem q x: (x == x) = (Atom {| ps := en 0; psv := 2 |} [x; x]).
 Proof. reflexivity. Defined.
 
+Definition p2_23_a ctx (t:Terms) (*x:SetVars.t*): APR ctx (t == t).
+pose (x:=0).
 Proof. 
-apply MP with (A:= Fora x (x == x)).
+(*apply MP with (A:= Fora x (x == x)).
+change (Atom {| ps := en 0; psv := 2 |} [FVC x; FVC x]) with (x == x).
+*)
+apply MP with (A:= Fora x ( x == x)).
 (*
 try fold (Fora x (x == x)).
 try rewrite <- q.
 pose (q:= (x == x)).
 replace (Atom {| ps := en 0; psv := 2 |} [FVC x; FVC x]) with (x == x).
 *)
-apply GEN.
+(*apply GEN.*)
 apply Hax, (aeq1 x).
 apply Hax, aPC.
 apply Ha12 with (t:=t).
@@ -80,9 +88,23 @@ simpl.
 rewrite -> Facts.eqb_refl.
 reflexivity.
 Defined.
-Definition p2_23_b ctx (t s:Terms) (x:SetVars.t):
+
+(*TODO Prove the completeness theorem. *)
+Definition swap ctx A B C: 
+(PR ctx (A --> (B --> C) --> (B --> (A --> C)) )).
+Proof.
+Fail Check Ded.
+Fail intro b.
+Admitted.
+Definition p2_23_b ctx (t s:Terms) (x y:SetVars.t):
 APR ctx ((t==s) --> (s==t) ).
 Proof.
+pose (step1 := aeq2 x y (y == x) (x == x)).
+pose (step2 := swap ctx (x == y) (x == x) (y == x)).
+(*Check MP _ ctx (x == x) ((x == y) --> (y == x)). *)
+(*apply MP with .
+apply MP with (A:= Fora x (x == x)).
+apply aeq2.*)
 
 Abort.
 End inf_sec.
